mem/Mem1.v
@@ -7,6 +7,7 @@ Require Import ModSem.
 Require Import Skeleton.
 Require Import PCM.
 Require Import Hoare.
+Require Import TODOYJ.
 
 Generalizable Variables E R A B C X Y Σ.
 
@@ -15,18 +16,6 @@ Set Implicit Arguments.
 
 
 
-(* Definition until (n: nat): list nat := mapi (fun n _ => n) (List.repeat tt n). *)
-
-
-(*** TODO: move to Coqlib ***)
-Definition map_fst A B C (f: A -> C): A * B -> C * B := fun '(a, b) => (f a, b).
-Definition map_snd A B C (f: B -> C): A * B -> A * C := fun '(a, b) => (a, f b).
-
-
-(** TODO: move to PCM.v **)
-Declare Scope ra_scope.
-Delimit Scope ra_scope with ra.
-Notation " K ==> V' " := (URA.pointwise K V'): ra_scope.
 
 
 
@@ -35,40 +24,69 @@ Compute (URA.car (t:=_memRA)).
 Instance memRA: URA.t := URA.auth _memRA.
 Compute (URA.car).
 
-Definition points_to (loc: block * Z) (v: val): URA.car :=
-  let (b, ofs) := loc in
-  URA.white (M:=_memRA)
-            (fun _b _ofs => if (dec _b b) && (dec _ofs ofs) then inl (Some v) else inr tt).
-
-Definition points_tos (loc: block * Z) (vs: list val): URA.car :=
-  let (b, ofs) := loc in
-  URA.white (M:=_memRA)
-            (fun _b _ofs => if (dec _b b) && ((ofs <=? _ofs) && (_ofs <? (ofs + Z.of_nat (List.length vs))))%Z
-                            then inl (List.nth_error vs (Z.to_nat (_ofs - ofs))) else inr tt).
-
-
-
-
-(* Definition own {GRA: GRA.t} (whole a: URA.car (t:=GRA)): Prop := URA.extends a whole. *)
-
-Notation "loc |-> v" := (points_to loc v) (at level 20).
-
-
-
-
 
 Section PROOF.
-  Context {Σ: GRA.t}.
-  (*** TODO: move to proper place, together with "mk_simple" ***)
-  (*** TODO: rename sb into spb ***)
-  (*** TODO: remove redundancy with Hoareproof0.v ***)
-  Definition mk_simple (mn: string) {X: Type} (P: X -> Any.t -> Σ -> ord -> Prop) (Q: X -> Any.t -> Σ -> Prop): fspec :=
-    @mk _ mn X (list val) (val) (fun x y a r o => P x a r o /\ y↑ = a) (fun x z a r => Q x a r /\ z↑ = a)
+  Context `{@GRA.inG memRA Σ}.
+  
+  Definition points_to (loc: block * Z) (vs: list val): Σ :=
+    let (b, ofs) := loc in
+    let memr: memRA := URA.white (M:=_memRA)
+                                 (fun _b _ofs => if (dec _b b) && ((ofs <=? _ofs) && (_ofs <? (ofs + Z.of_nat (List.length vs))))%Z
+                                                 then inl (List.nth_error vs (Z.to_nat (_ofs - ofs))) else inr tt) in
+    (GRA.padding memr)
   .
-  Definition mk_sb_simple (mn: string) {X: Type} (P: X -> Any.t -> Σ -> ord -> Prop) (Q: X -> Any.t -> Σ -> Prop)
-             (body: list val -> itree (hCallE +' pE +' eventE) val): fspecbody := mk_specbody (mk_simple mn P Q) body.
+
+  Lemma points_to_split
+        blk ofs hd tl
+    :
+      (points_to (blk, ofs) (hd :: tl)) = (points_to (blk, ofs) [hd]) ⋅ (points_to (blk, (ofs + 1)%Z) tl)
+  .
+  Proof.
+    ss. rewrite GRA.padding_add. repeat f_equal.
+    ss. unfold URA.white. f_equal.
+    repeat (apply func_ext; i).
+    des_ifs; bsimpl; des; des_sumbool; ss; try rewrite Z.leb_gt in *; try rewrite Z.leb_le in *;
+      try rewrite Z.ltb_ge in *; try rewrite Z.ltb_lt in *; try lia.
+    - clear_tac. subst. rewrite Zpos_P_of_succ_nat in *. rewrite <- Zlength_correct in *.
+      assert(x0 = ofs).
+      { lia. }
+      subst.
+      f_equal. rewrite Z.sub_diag. ss.
+    - clear_tac. subst. rewrite Zpos_P_of_succ_nat in *. rewrite <- Zlength_correct in *.
+      f_equal. clear Heq4. clear Heq5. clear_tac.
+      destruct (Z.to_nat (x0 - ofs)) eqn:T; ss.
+      { exfalso. lia. }
+      f_equal. lia.
+  Qed.
+
+(* Lemma points_tos_points_to *)
+(*       loc v *)
+(*   : *)
+(*     (points_to loc v) = (points_tos loc [v]) *)
+(* . *)
+(* Proof. *)
+(*   apply func_ext. i. *)
+(*   apply prop_ext. *)
+(*   ss. split; i; r. *)
+(*   - des_ifs. ss. eapply Own_extends; et. rp; try refl. repeat f_equal. repeat (apply func_ext; i). *)
+(*     des_ifs; bsimpl; des; des_sumbool; ss; clarify. *)
+(*     + rewrite Z.sub_diag; ss. *)
+(*     + rewrite Z.leb_refl in *; ss. *)
+(*     + rewrite Z.ltb_ge in *. lia. *)
+(*     + rewrite Z.ltb_lt in *. lia. *)
+(*   - des_ifs. ss. eapply Own_extends; et. rp; try refl. repeat f_equal. repeat (apply func_ext; i). *)
+(*     des_ifs; bsimpl; des; des_sumbool; ss; clarify. *)
+(*     + rewrite Z.sub_diag; ss. *)
+(*     + rewrite Z.ltb_lt in *. lia. *)
+(*     + rewrite Z.leb_refl in *; ss. *)
+(*     + rewrite Z.ltb_ge in *. lia. *)
+(* Qed. *)
 
 End PROOF.
+
+Notation "loc |-> vs" := (points_to loc vs) (at level 20).
+
+
 
 
 
@@ -77,152 +95,58 @@ Section PROOF.
   Let GURA: URA.t := GRA.to_URA Σ.
   Local Existing Instance GURA.
 
-  (* Definition mem_inv: Σ -> Prop := *)
-  (*   fun mr0 => exists mem0, mr0 = GRA.padding (URA.black (M:=_memRA) (inl mem0)). *)
-
-
-  (*** TODO: morally, we want:
-```
-      sz <- trigger (Take nat);;
-      assume(varg = [Vint (Z.of_nat sz)]);;
-```
-  ***)
-
-
-  (* Definition allocF: list val -> itree Es val := *)
-  (*   HoareFun "Mem" *)
-  (*            (fun sz varg _ => varg = [Vint (Z.of_nat sz)]) *)
-  (*            (fun sz vret rret => *)
-  (*               exists b, vret = Vptr b 0 /\ *)
-  (*               rret = GRA.padding (fold_left URA.add (mapi (fun n _ => (b, Z.of_nat n) |-> (Vint 0)) *)
-  (*                                                           (List.repeat tt sz)) URA.unit)) *)
-  (*            (fun _ => trigger (Choose _)) *)
-  (* . *)
-
-  (* Definition freeF: list val -> itree Es val := *)
-  (*   HoareFun "Mem" *)
-  (*            (fun '(b, ofs, v) varg rarg => varg = [Vptr b ofs] /\ *)
-  (*                                           rarg = (GRA.padding ((b, ofs) |-> v))) *)
-  (*            (top3) *)
-  (*            (fun _ => trigger (Choose _)) *)
-  (* . *)
-
-  (* Definition loadF: list val -> itree Es val := *)
-  (*   HoareFun "Mem" *)
-  (*            (fun '(b, ofs, v) varg rarg => varg = [Vptr b ofs] /\ *)
-  (*                                           rarg = (GRA.padding ((b, ofs) |-> v))) *)
-  (*            (fun '(b, ofs, v) vret rret => rret = (GRA.padding ((b, ofs) |-> v)) /\ vret = v) *)
-  (*            (fun _ => trigger (Choose _)) *)
-  (* . *)
-
-  (* Definition storeF: list val -> itree Es val := *)
-  (*   HoareFun "Mem" *)
-  (*            (fun '(b, ofs, v_old, v_new) varg rarg => *)
-  (*               varg = [Vptr b ofs ; v_new] /\ rarg = (GRA.padding ((b, ofs) |-> v_old))) *)
-  (*            (fun '(b, ofs, v_old, v_new) _ rret => rret = (GRA.padding ((b, ofs) |-> v_new))) *)
-  (*            (fun _ => trigger (Choose _)) *)
-  (* . *)
-
   Let alloc_spec: fspec := (mk_simple "Mem"
-                                      (fun sz varg _ o => varg = [Vint (Z.of_nat sz)]↑ /\ o = ord_pure 1)
+                                      (fun sz varg o _ => varg = [Vint (Z.of_nat sz)]↑ /\ o = ord_pure 1)
                                       (fun sz vret rret =>
                                          exists b, vret = (Vptr b 0)↑ /\
-                                                   rret = GRA.padding (points_tos (b, 0%Z) (List.repeat (Vint 0) sz)))).
+                                                   rret = (points_to (b, 0%Z) (List.repeat (Vint 0) sz)))).
 
   Let free_spec: fspec := (mk_simple "Mem"
-                                     (fun '(b, ofs) varg rarg o => exists v, varg = ([Vptr b ofs])↑ /\
-                                                                             rarg = (GRA.padding ((b, ofs) |-> v)) /\
+                                     (fun '(b, ofs) varg o rarg => exists v, varg = ([Vptr b ofs])↑ /\
+                                                                             rarg = ((b, ofs) |-> [v]) /\
                                                                              o = ord_pure 1)
                                      (top3)).
 
   Let load_spec: fspec := (mk_simple "Mem"
-                                     (fun '(b, ofs, v) varg rarg o => varg = ([Vptr b ofs])↑ /\
-                                                                      rarg = (GRA.padding ((b, ofs) |-> v)) /\
+                                     (fun '(b, ofs, v) varg o rarg => varg = ([Vptr b ofs])↑ /\
+                                                                      rarg = ((b, ofs) |-> [v]) /\
                                                                       o = ord_pure 1)
-                                     (fun '(b, ofs, v) vret rret => rret = (GRA.padding ((b, ofs) |-> v)) /\ vret = v↑)).
+                                     (fun '(b, ofs, v) vret rret => rret = ((b, ofs) |-> [v]) /\ vret = v↑)).
 
   Let store_spec: fspec := (mk_simple
                               "Mem"
-                              (fun '(b, ofs, v_new) varg rarg o => exists v_old,
-                                   varg = ([Vptr b ofs ; v_new])↑ /\ rarg = (GRA.padding ((b, ofs) |-> v_old)) /\ o = ord_pure 1)
-                              (fun '(b, ofs, v_new) _ rret => rret = (GRA.padding ((b, ofs) |-> v_new)))).
+                              (fun '(b, ofs, v_new) varg o rarg => exists v_old,
+                                   varg = ([Vptr b ofs ; v_new])↑ /\ rarg = ((b, ofs) |-> [v_old]) /\ o = ord_pure 1)
+                              (fun '(b, ofs, v_new) _ rret => rret = ((b, ofs) |-> [v_new]))).
+
+  Let cmp_spec: fspec :=
+    (mk_simple
+       "Mem"
+       (fun '(result, resource) varg o rarg =>
+          rarg = resource /\
+          ((exists b ofs v, varg = [Vptr b ofs; Vnullptr]↑ /\ rarg = ((b, ofs) |-> v) /\ result = false) \/
+           (exists b0 ofs0 v0 b1 ofs1 v1, varg = [Vptr b0 ofs0; Vptr b1 ofs1]↑ /\ rarg = ((b0, ofs0) |-> v0) ⋅ ((b1, ofs1) |-> v1) /\ result = false) \/
+           (exists b ofs v, varg = [Vptr b ofs; Vptr b ofs]↑ /\ rarg = ((b, ofs) |-> v) /\ result = true)
+          )
+       )
+       (fun '(result, resource) varg rret => varg = result↑ /\ rret = resource)
+    ).
 
   Definition MemStb: list (gname * fspec) :=
-    [("alloc", alloc_spec) ; ("free", free_spec) ; ("load", load_spec) ; ("store", store_spec)]
+    [("alloc", alloc_spec) ; ("free", free_spec) ; ("load", load_spec) ; ("store", store_spec) ; ("cmp", cmp_spec)]
   .
 
   Definition MemSbtb: list (gname * fspecbody) :=
     [("alloc", mk_specbody alloc_spec (fun _ => trigger (Choose _)));
     ("free",   mk_specbody free_spec (fun _ => trigger (Choose _)));
     ("load",   mk_specbody load_spec (fun _ => trigger (Choose _)));
-    ("store",   mk_specbody store_spec (fun _ => trigger (Choose _)))
+    ("store",  mk_specbody store_spec (fun _ => trigger (Choose _)));
+    ("cmp",    mk_specbody cmp_spec (fun _ => trigger (Choose _)))
     ]
   .
 
-
-
-
-
-
-  (* Definition MemSbtb: list (gname * fspecbody) := *)
-  (* [("alloc", mk_sb_simple "Mem" *)
-  (*              (fun sz varg _ => varg = [Vint (Z.of_nat sz)]↑) *)
-  (*              (fun sz vret rret => *)
-  (*                 exists b, vret = (Vptr b 0)↑ /\ *)
-  (*                           rret = GRA.padding (points_tos (b, 0%Z) (List.repeat (Vint 0) sz))) *)
-  (*              (fun _ => (ord_pure 1)) *)
-  (*              (fun _ => trigger (Choose _))) ; *)
-  (* ("free", mk_sb_simple "Mem" *)
-  (*             (fun '(b, ofs) varg rarg => exists v, varg = ([Vptr b ofs])↑ /\ *)
-  (*                                                   rarg = (GRA.padding ((b, ofs) |-> v))) *)
-  (*             (top3) *)
-  (*             (fun _ => (ord_pure 1)) *)
-  (*             (fun _ => trigger (Choose _))) ; *)
-  (* ("load", mk_sb_simple "Mem" *)
-  (*             (fun '(b, ofs, v) varg rarg => varg = ([Vptr b ofs])↑ /\ *)
-  (*                                          rarg = (GRA.padding ((b, ofs) |-> v))) *)
-  (*             (fun '(b, ofs, v) vret rret => rret = (GRA.padding ((b, ofs) |-> v)) /\ vret = v↑) *)
-  (*             (fun _ => (ord_pure 1)) *)
-  (*             (fun _ => trigger (Choose _))) ; *)
-  (* ("store", mk_sb_simple *)
-  (*             "Mem" *)
-  (*              (fun '(b, ofs, v_new) varg rarg => exists v_old, *)
-  (*                   varg = ([Vptr b ofs ; v_new])↑ /\ rarg = (GRA.padding ((b, ofs) |-> v_old))) *)
-  (*              (fun '(b, ofs, v_new) _ rret => rret = (GRA.padding ((b, ofs) |-> v_new))) *)
-  (*              (fun _ => (ord_pure 1)) *)
-  (*              (fun _ => trigger (Choose _))) *)
-  (* ] *)
-  (* . *)
-
-  (* Definition MemStb: list (gname * fspec) := List.map (map_snd fsb_fspec) MemSbtb. *)
-
-  (* Definition MemFtb2: list (gname * fspec * (list val -> itree (hCallE +' eventE) val)) := *)
-  (* [("alloc", mk "Mem" *)
-  (*              (fun sz varg _ => varg = [Vint (Z.of_nat sz)]) *)
-  (*              (fun sz vret rret => *)
-  (*                 exists b, vret = Vptr b 0 /\ *)
-  (*                           rret = GRA.padding (fold_left URA.add *)
-  (*                                                         (mapi (fun n _ => (b, Z.of_nat n) |-> (Vint 0)) *)
-  (*                                                               (List.repeat tt sz)) URA.unit)), (fun _ => trigger (Choose _))) ; *)
-  (* ("free", mk "Mem" *)
-  (*             (fun '(b, ofs, v) varg rarg => varg = [Vptr b ofs] /\ *)
-  (*                                            rarg = (GRA.padding ((b, ofs) |-> v))) *)
-  (*             (top3), (fun _ => trigger (Choose _))) ; *)
-  (* ("load", mk "Mem" *)
-  (*             (fun '(b, ofs, v) varg rarg => varg = [Vptr b ofs] /\ *)
-  (*                                            rarg = (GRA.padding ((b, ofs) |-> v))) *)
-  (*             (fun '(b, ofs, v) vret rret => rret = (GRA.padding ((b, ofs) |-> v)) /\ vret = v), (fun _ => trigger (Choose _))) ; *)
-  (* ("store", mk "Mem" *)
-  (*              (fun '(b, ofs, v_old, v_new) varg rarg => *)
-  (*                 varg = [Vptr b ofs ; v_new] /\ rarg = (GRA.padding ((b, ofs) |-> v_old))) *)
-  (*              (fun '(b, ofs, v_old, v_new) _ rret => rret = (GRA.padding ((b, ofs) |-> v_new))), (fun _ => trigger (Choose _))) *)
-  (* ] *)
-  (* . *)
-  (* Goal MemFtb = MemFtb2. refl. Qed. *)
-
   Definition MemSem: ModSem.t := {|
     ModSem.fnsems := List.map (fun '(fn, fsb) => (fn, fun_to_tgt MemStb fn fsb)) MemSbtb;
-      (* [("alloc", allocF) ; ("free", freeF) ; ("load", loadF) ; ("store", storeF)]; *)
     ModSem.initial_mrs := [("Mem", (GRA.padding (URA.black (M:=_memRA) (fun _ _ => inr tt)), unit↑))];
   |}
   .
