examples/delayed_echo/TODOYJ.v
@@ -1,0 +1,193 @@
+Require Import Coqlib.
+Require Import ITreelib.
+Require Import Universe.
+Require Import STS.
+Require Import Behavior.
+Require Import ModSem.
+Require Import Skeleton.
+Require Import PCM.
+Require Import Hoare.
+
+Generalizable Variables E R A B C X Y Σ.
+
+Set Implicit Arguments.
+Set Typeclasses Depth 5.
+
+
+
+
+Global Opaque GRA.to_URA.
+Infix "⋅" := URA.add (at level 50, left associativity).
+Notation "(⋅)" := URA.add (only parsing).
+
+
+Definition unleftU {E X Y} `{eventE -< E} (xy: X + Y): itree E X :=
+  match xy with
+  | inl x => Ret x
+  | inr y => triggerUB
+  end.
+
+Definition unleftN {E X Y} `{eventE -< E} (xy: X + Y): itree E X :=
+  match xy with
+  | inl x => Ret x
+  | inr y => triggerNB
+  end.
+
+Definition unrightU {E X Y} `{eventE -< E} (xy: X + Y): itree E Y :=
+  match xy with
+  | inl x => triggerUB
+  | inr y => Ret y
+  end.
+
+Definition unrightN {E X Y} `{eventE -< E} (xy: X + Y): itree E Y :=
+  match xy with
+  | inl x => triggerNB
+  | inr y => Ret y
+  end.
+
+Section UNPADDING.
+  
+  Definition unpadding A {Σ} `{@GRA.inG A Σ} (a: URA.car (t:=Σ)): itree Es (URA.car (t:=A)) :=
+    assume(forall n (NEQ: n <> GRA.inG_id), a n = URA.unit);;
+    Ret (eq_rect_r (@URA.car) (a GRA.inG_id) GRA.inG_prf)
+  .
+
+  Definition unpadding2 {A Σ} `{@GRA.inG A Σ} (a: URA.car (t:=Σ)): itree Es (URA.car (t:=A)) :=
+    n <- trigger (Choose _);;
+    (if Nat.eq_dec GRA.inG_id n
+     then Ret tt
+     else  assume (a n = URA.unit);; Ret tt);;
+    Ret (eq_rect_r (@URA.car) (a GRA.inG_id) GRA.inG_prf)
+  .
+
+End UNPADDING.
+Arguments unpadding _ {Σ H}.
+
+
+
+
+
+
+
+
+
+
+
+
+
+
+
+
+Section PROOF.
+  Context {Σ: GRA.t}.
+  (*** TODO: move to proper place, together with "mk_simple" ***)
+  (*** TODO: rename sb into spb ***)
+  (*** TODO: remove redundancy with Hoareproof0.v ***)
+  Definition mk_simple (mn: string) {X: Type} (P: X -> Any.t -> ord -> Σ -> Prop) (Q: X -> Any.t -> Σ -> Prop): fspec :=
+    @mk _ mn X (list val) (val) (fun x y a r o => P x a o r /\ y↑ = a) (fun x z a r => Q x a r /\ z↑ = a)
+  .
+  Definition mk_sb_simple (mn: string) {X: Type} (P: X -> Any.t -> ord -> Σ -> Prop) (Q: X -> Any.t -> Σ -> Prop)
+             (body: list val -> itree (hCallE +' pE +' eventE) val): fspecbody := mk_specbody (mk_simple mn P Q) body.
+
+End PROOF.
+
+
+
+
+
+
+Section IRIS.
+  Context {Σ: GRA.t}.
+  Definition iProp := Σ -> Prop.
+  Definition Sepconj (P Q: iProp): iProp :=
+    fun r => exists a b, r = URA.add a b /\ P a /\ Q b
+  .
+  Definition Pure (P: Prop): iProp := fun _ => P.
+  Definition Ex {X: Type} (P: X -> iProp): iProp := fun r => exists x, P x r.
+  Definition Own (r0: Σ): iProp := fun r1 => URA.extends r0 r1.
+  (* Definition Own (r0: Σ): iProp := fun r1 => r0 = r1. *)
+
+  Definition Impl (P Q: iProp): Prop := P <1= Q.
+  Infix "i->" := Impl (at level 60).
+  Notation "P 'i<->' Q" := ((Impl P Q) /\ (Impl Q P)) (at level 60).
+
+  Lemma Own_extends
+        (a b: Σ)
+        (EXT: URA.extends a b)
+    :
+      (Own b) i-> (Own a)
+  .
+  Proof. ii. ss. r in PR. r. etrans; et. Qed.
+
+  Lemma Iff_eq
+        P Q
+        (IFF: P i<-> Q)
+    :
+      P = Q
+  .
+  Proof.
+    apply func_ext. i. apply prop_ext. des. split; i; et.
+  Qed.
+
+  Lemma own_sep'
+        (r0 r1 r2: Σ)
+        (ADD: r0 = r1 ⋅ r2)
+    :
+      Own r0 = Sepconj (Own r1) (Own r2)
+  .
+  Proof.
+    apply Iff_eq.
+    split; ii.
+    - clarify. r in PR. r. r in PR. des. exists r1, (r2 ⋅ ctx). esplits; et.
+      + rewrite URA.add_assoc. ss.
+      + refl.
+      + rr. esplits; et.
+    - r in PR. r. des. clarify. r in PR0. r in PR1. etrans.
+      { eapply URA.extends_add; et. }
+      rewrite ! (URA.add_comm a).
+      eapply URA.extends_add; et.
+  Qed.
+
+  Lemma own_sep
+        (r1 r2: Σ)
+    :
+      Own (r1 ⋅ r2) = Sepconj (Own r1) (Own r2)
+  .
+  Proof.
+    erewrite <- own_sep'; et.
+  Qed.
+
+End IRIS.
+
+Infix "**" := Sepconj (at level 60).
+Notation "'⌜' P '⌝'" := (Pure P).
+Notation "'Exists' x .. y , p" := (Ex (fun x => .. (Ex (fun y => p)) ..))
+                                    (at level 200, x binder, right associativity,
+                                     format "'[' 'Exists'  '/  ' x  ..  y ,  '/  ' p ']'").
+
+
+
+
+
+
+
+
+
+
+
+
+
+
+(* Definition until (n: nat): list nat := mapi (fun n _ => n) (List.repeat tt n). *)
+
+
+(*** TODO: move to Coqlib ***)
+Definition map_fst A B C (f: A -> C): A * B -> C * B := fun '(a, b) => (f a, b).
+Definition map_snd A B C (f: B -> C): A * B -> A * C := fun '(a, b) => (a, f b).
+
+
+(** TODO: move to PCM.v **)
+Declare Scope ra_scope.
+Delimit Scope ra_scope with ra.
+Notation " K ==> V' " := (URA.pointwise K V'): ra_scope.
+
