mem/Mem01proof.v
@@ -73,12 +73,21 @@ Section SIMMODSEM.
   Context `{Σ: GRA.t}.
   Context `{@GRA.inG Mem1.memRA Σ} `{@GRA.inG (RA.excl Mem.t) Σ}.
 
-  Let W: Type := (alist mname Σ) * (alist mname Σ).
+  Let W: Type := (alist mname (Σ * Any.t)) * (alist mname (Σ * Any.t)).
   (* Eval compute in (@RA.car (RA.excl Mem.t)). *)
   Eval compute in (@RA.car Mem1._memRA).
   Inductive sim_loc: option val -> (option val + unit) -> Prop :=
   | sim_loc_present v: sim_loc (Some v) (inl (Some v))
   | sim_loc_absent: sim_loc None (inr tt)
+  .
+
+  Let wf: W -> Prop :=
+    fun '(mrps_src0, mrps_tgt0) =>
+      exists mem_src (mem_tgt: Mem.t),
+        (<<SRC: mrps_src0 = Maps.add "Mem" ((GRA.padding ((URA.black mem_src): URA.car (t:=Mem1.memRA))), tt↑) Maps.empty>>) /\
+        (<<TGT: mrps_tgt0 = Maps.add "Mem" (ε, mem_tgt↑) Maps.empty>>) /\
+        (<<SIM: forall b ofs, sim_loc ((mem_tgt.(Mem.cnts)) b ofs) (mem_src b ofs)>>) /\
+        (<<NULLPTR: >>)
   .
 
   Let wf: W -> Prop :=
@@ -95,9 +104,340 @@ Section SIMMODSEM.
   Infix "⋅" := URA.add (at level 50, left associativity).
   Notation "(⋅)" := URA.add (only parsing).
 
-  Local Opaque points_tos.
+  Local Opaque points_to.
   Theorem correct: ModSemPair.sim Mem1.MemSem Mem0.MemSem.
-  Proof. admit "fix it later -- after the some tooling is developed". Qed.
+  Proof.
+    econstructor 1 with (wf:=wf) (le:=top2); et; swap 2 3.
+    { typeclasses eauto. }
+    { ss. esplits; ss; et. ii. econs 2. }
+    econs; ss.
+    { split; ss. ii; clarify. rename y into varg. eexists 100%nat. ss. des; clarify.
+      unfold alist_add, alist_remove; ss.
+      unfold Mem0.allocF.
+      (* Opaque MemStb. *)
+      (* Opaque mapi. *)
+      Local Opaque URA.add.
+      go. ss. rename x into sz.
+      unfold assume.
+      igo.
+      go. clarify. unfold HoareFun. go. rename x into rarg_src.
+      unfold assume.
+      igo.
+      repeat go. clear_tac.
+      Opaque URA.add.
+      unfold unpadding, assume.
+      igo.
+      pfold. econsr; et. esplits; et. left.
+      igo. des_ifs.
+      unfold unwrapU. des_ifs. igo. des_ifs. unfold MPut. igo. repeat go.
+      ss. clarify.
+      force_r. esplits; ss. left.
+      go. igo.
+      go. igo.
+      Hint Unfold alist_add.
+      u.
+      Hint Unfold body_to_tgt interp_hCallE_tgt.
+      u. igo.
+      Local Opaque MemStb.
+      cbn.
+      set (blk := (Mem.nb mem_tgt)) in *.
+      force_l. exists (Vptr (Mem.nb mem_tgt) 0). left.
+      igo. go.
+      force_l.
+      set (mem_src_new := add_delta_to_black
+                            (* (URA.excl (mem_src: URA.car (t:=Mem1._memRA)) frag) *)
+                            (URA.black (mem_src: URA.car (t:=Mem1._memRA)))
+                            (points_tos (blk, 0%Z) (repeat (Vint 0) sz))).
+      eexists (GRA.padding (mem_src_new: URA.car (t:=Mem1.memRA)),
+               GRA.padding (points_tos (blk, 0%Z) (repeat (Vint 0) sz))). left.
+      igo. force_l.
+      {
+        replace (fun k => URA.unit) with (URA.unit (t:=Σ)) by ss.
+        rewrite URA.unit_idl.
+        rewrite GRA.padding_add.
+        rewrite <- URA.unit_id.
+        apply URA.updatable_add; cycle 1.
+        { apply URA.updatable_unit. }
+        eapply GRA.padding_updatable.
+        subst mem_src_new. des_ifs.
+        ss. clarify.
+        rewrite <- Heq.
+        Local Transparent points_tos.
+        replace ((fun _ _ => @inr (option val) unit tt)) with (URA.unit (t:=Mem1._memRA)) by ss.
+        replace (URA.excl ((mem_src: URA.car (t:=Mem1._memRA)) ⋅ f) URA.unit) with
+            (URA.black ((mem_src: URA.car (t:=Mem1._memRA)) ⋅ f)) by ss.
+        rewrite Heq.
+        eapply URA.auth_alloc2.
+
+        clear - WF Heq SIM.
+        { ss. intros b ofs. des_ifs. ss.
+
+          assert(WF0: URA.wf ((GRA.padding (URA.black (mem_src: URA.car (t:=Mem1._memRA))))
+                                ⋅ (URA.unit ⋅ (rarg_src: URA.car (t:=GRA.to_URA Σ))))).
+          { ss. }
+          eapply URA.wf_mon in WF0.
+          eapply GRA.padding_wf in WF0.
+
+          unfold URA.white in *. clarify.
+          subst blk.
+          Local Transparent URA.add.
+          ss. des_ifs.
+          - bsimpl; des; des_sumbool; clarify.
+            admit "ez: Heq is wrong. Add mem tgt is wf (nb is actually nb); use sim_loc.".
+          - des. specialize (WF1 b ofs). bsimpl; des; des_sumbool; clarify; des_ifs.
+          - des. specialize (WF1 b ofs). bsimpl; des; des_sumbool; clarify; des_ifs.
+            apply_all_once Z.leb_le. apply_all_once Z.ltb_lt.
+            intro A. apply nth_error_None in A. rewrite repeat_length in *.
+            apply inj_le in A. rewrite Z2Nat.id in A; cycle 1.
+            { lia. }
+            lia.
+        }
+      }
+      left.
+      force_l. eexists. left.
+      unfold guarantee. igo.
+      force_l. esplits; et. left.
+      Local Opaque add_delta_to_black.
+      pfold; econs; try (by ss).
+      { instantiate (1:= GRA.padding _). rewrite GRA.padding_add. rewrite URA.unit_idl. f_equal. }
+      left.
+      pfold; econs; ss; et.
+      {
+        rr. unfold alist_add. ss. esplits; ss; et.
+        { unfold mem_src_new.
+          Local Transparent add_delta_to_black.
+          ss.
+        }
+        ii. ss.
+        subst mem_src_new.
+        assert(b <> blk).
+        {admit "should be ez". }
+        hexploit (SIM b ofs); et. intro A. inv A.
+        {
+          des_ifs; bsimpl; des; des_sumbool; clarify.
+          - unfold update. des_ifs. rewrite <- H3. econs.
+          - unfold update. des_ifs. rewrite <- H3. econs.
+          - unfold update. des_ifs. rewrite <- H3. econs.
+        }
+        {
+          des_ifs; bsimpl; des; des_sumbool; clarify.
+          - unfold update. des_ifs. rewrite <- H3. econs.
+          - unfold update. des_ifs. rewrite <- H3. econs.
+          - unfold update. des_ifs. rewrite <- H3. econs.
+        }
+      }
+    }
+    econs.
+    { split; ss. ii; clarify. rename y into varg. eexists 100%nat. ss. des; clarify.
+      u.
+      unfold Mem0.freeF.
+      Local Opaque URA.add.
+      go. ss. destruct x as [b ofs].
+      unfold assume.
+      igo.
+      repeat (go; igo). des; clarify.
+      replace ((fun k => URA.unit): URA.car (t:=Σ))  with (URA.unit: URA.car (t:=Σ)) in WF by ss.
+      rewrite URA.unit_idl in WF.
+      rewrite GRA.padding_add in WF. apply GRA.padding_wf in WF. des.
+      Local Opaque URA.wf.
+      Hint Unfold handle_hCallE_tgt.
+      u. igo. ss.
+      force_l. eexists (Vint 0). left.
+      repeat (go; igo).
+      force_r. eexists. left.
+      repeat (go; igo).
+      force_r. esplits; et. left.
+      assert(A: mem_src b ofs = inl (Some v)).
+      {
+        Local Transparent URA.wf.
+        ss. des_ifs. des. specialize (WF0 b ofs).
+        Local Transparent URA.add.
+        clear SIM.
+        ss. clarify. rr in WF. des. clarify. ss. des_ifs.
+        - bsimpl; des; des_sumbool; ss.
+        - bsimpl; des; des_sumbool; ss.
+      }
+      Local Opaque URA.wf.
+      Local Opaque URA.add.
+      hexploit (SIM b ofs); et. intro B. rewrite A in *. inv B.
+      unfold unwrapU. des_ifs; cycle 1.
+      {exfalso. unfold Mem.free in *. des_ifs. }
+      repeat (igo; go).
+      unfold MPut.
+      repeat (igo; go).
+      u.
+      set (mem_src' := fun _b _ofs => if dec _b b && dec _ofs ofs then inr () else mem_src _b _ofs).
+      assert(WF': URA.wf (mem_src': URA.car (t:=Mem1._memRA))).
+      { Local Transparent URA.wf.
+        Local Transparent URA.add.
+        ss. ii. des_ifs.
+        ss. clarify.
+        subst mem_src'. ss. des_ifs. des. specialize (WF0 k k0). bsimpl. des; des_sumbool; des_ifs.
+        Local Opaque URA.wf.
+        Local Opaque URA.add.
+      }
+      rename t into mem_tgt'.
+      assert(SIM': forall b ofs, sim_loc (Mem.cnts mem_tgt' b ofs) (mem_src' b ofs)).
+      { i.
+        unfold Mem.free in Heq. des_ifs. ss.
+        subst mem_src'. ss.
+        destruct (classic (b = b0 /\ ofs = ofs0)); des; clarify.
+        - unfold update. des_ifs. econs.
+        - des_ifs.
+          { Psimpl. bsimpl; des; des_sumbool; ss; clarify. }
+          replace (update (Mem.cnts mem_tgt) b (update (Mem.cnts mem_tgt b) ofs None) b0 ofs0) with
+              (Mem.cnts mem_tgt b0 ofs0); cycle 1.
+          { unfold update. des_ifs. Psimpl. des_ifs; bsimpl; des; des_sumbool; ss; clarify. }
+          et.
+      }
+      force_l.
+      eexists ((GRA.padding (URA.black (mem_src': URA.car (t:=Mem1._memRA)))), URA.unit: URA.car (t:=Σ)). left.
+      force_l.
+      { replace (fun k => URA.unit) with (URA.unit: URA.car (t:=Σ)) by ss.
+        rewrite URA.unit_id. rewrite URA.unit_idl.
+        rewrite GRA.padding_add. apply GRA.padding_updatable.
+        apply URA.auth_dealloc.
+        clear - WF' WF.
+        r. i. rewrite URA.unit_idl.
+        ss. destruct H; clear H. (*** coq bug; des infloops ***) des. clarify.
+        esplits; et.
+        apply func_ext. intro _b. apply func_ext. intro _ofs.
+        destruct (classic (b = _b /\ ofs = _ofs)).
+        - destruct H; clear H. clarify.
+          subst mem_src'. ss. des_ifs; bsimpl; des; des_sumbool; clarify.
+          clear - H0.
+          Local Transparent URA.wf.
+          Local Transparent URA.add.
+          specialize (H0 _b _ofs). ss. des_ifs; bsimpl; des; des_sumbool; clarify. des_u. ss.
+        - Psimpl.
+          subst mem_src'. s. des_ifs; bsimpl; des; des_sumbool; clarify.
+          destruct H; clear H; des; clarify.
+          Local Opaque URA.wf.
+          Local Opaque URA.add.
+      }
+      left. u.
+      force_l. exists (URA.unit: URA.car (t:=Σ)). left.
+      unfold guarantee.
+      igo. force_l. esplits; et. left.
+      force_l.
+      { rewrite URA.unit_idl. ss. }
+      left.
+      pfold; econs; et.
+      ss.
+      esplits; ss; et.
+    }
+    Local Opaque GRA.to_URA.
+    Local Opaque points_to.
+    Local Opaque URA.add.
+    Local Opaque URA.wf.
+    econs.
+    { split; ss. ii; clarify. rename y into varg. eexists 100%nat. ss. des; clarify.
+      u.
+      unfold Mem0.loadF.
+      go. ss. destruct x as [[b ofs] v].
+      unfold assume.
+      igo.
+      repeat (go; igo). des_ifs. des; clarify. ss. rewrite URA.unit_idl in *.
+      rewrite GRA.padding_add in WF. apply GRA.padding_wf in WF. des.
+      Hint Unfold handle_hCallE_tgt.
+      u. igo. ss.
+      force_l. eexists _. left.
+      repeat (go; igo).
+      force_r. eexists. left.
+      repeat (go; igo).
+      force_r. esplits; et. left.
+      force_l. eexists (GRA.padding (URA.black (mem_src: URA.car (t:=Mem1._memRA))),
+                        GRA.padding ((b, ofs) |-> v)). left.
+      force_l. esplits; et. left.
+      force_l. esplits; et. left.
+      unfold guarantee.
+      repeat (go; igo).
+      force_l. esplits; et. left.
+      force_l. { rewrite URA.unit_idl; refl. } left.
+      Local Transparent URA.wf.
+      Local Transparent URA.add.
+      Local Transparent GRA.to_URA.
+      Local Transparent points_to.
+      ss. des_ifs. des; ss. do 2 spc WF0. des_ifs; cycle 1.
+      { exfalso. rr in WF. des. ss. des_ifs. do 2 spc SIM. des_ifs. bsimpl; des; des_sumbool; ss. }
+      destruct o; ss.
+      assert(v0 = v).
+      { rr in WF. des. ss. des_ifs. do 2 spc SIM. des_ifs. bsimpl; des; des_sumbool; ss. }
+      clarify.
+      unfold unwrapU. unfold Mem.load. exploit SIM; et. intro T. rewrite Heq in *. inv T.
+      pfold. econs; et.
+      rr. esplits; ss; et.
+    }
+    Local Opaque GRA.to_URA.
+    Local Opaque points_to.
+    Local Opaque URA.add.
+    Local Opaque URA.wf.
+    econs; et.
+    { split; ss. ii; clarify. rename y into varg. eexists 100%nat. ss. des; clarify.
+      u.
+      unfold Mem0.storeF.
+      go. ss. destruct x as [[b ofs] v].
+      set (mem_src' := fun _b _ofs => if dec _b b && dec _ofs ofs then inl (Some v) else mem_src _b _ofs).
+      unfold assume.
+      igo.
+      repeat (go; igo). des_ifs. des; clarify. ss. rewrite URA.unit_idl in *.
+      rewrite GRA.padding_add in WF. apply GRA.padding_wf in WF. des.
+      Hint Unfold handle_hCallE_tgt.
+      u. igo. ss.
+      force_l. eexists _. left.
+      repeat (go; igo).
+      force_r. eexists. left.
+      repeat (go; igo).
+      force_r. esplits; et. left.
+      force_l. eexists (GRA.padding (URA.black (mem_src': URA.car (t:=Mem1._memRA))),
+                        GRA.padding ((b, ofs) |-> v)). left.
+      assert(WF0: URA.wf (mem_src': URA.car (t:=Mem1._memRA))).
+      { Local Transparent URA.wf.
+        clear - WF. apply URA.wf_mon in WF. ss. des.
+        ii. specialize (WF0 k k0). des_ifs_safe. unfold mem_src' in *. des_ifs.
+        Local Opaque URA.wf.
+      }
+      force_l.
+      { rewrite ! GRA.padding_add. eapply GRA.padding_updatable.
+        clear - WF WF0. clear WF.
+        Local Transparent URA.add GRA.to_URA points_to URA.wf.
+        eapply URA.auth_update; et.
+        rr. ii. destruct H; clear H. (*** FIXME: des runs infloop ***)
+        des. subst. esplits; et.
+        subst mem_src'. do 2 (apply func_ext; i). specialize (H0 x x0). specialize (WF0 x x0).
+        ss. des_ifs.
+        Local Opaque URA.add GRA.to_URA points_to URA.wf.
+      }
+      left.
+      force_l. esplits; et. left.
+      unfold guarantee.
+      repeat (go; igo).
+      force_l. esplits; et. left.
+      force_l. { rewrite URA.unit_idl; refl. } left.
+      assert(U: mem_src b ofs = inl (Some v_old)).
+      { Local Transparent URA.add GRA.to_URA points_to URA.wf.
+        clear - WF. ss. des. specialize (WF0 b ofs). r in WF. des; clarify. ss. des_ifs; ss.
+        - bsimpl; des; des_sumbool; ss.
+        - bsimpl; des; des_sumbool; ss.
+        Local Opaque URA.add GRA.to_URA points_to URA.wf.
+      }
+      hexploit SIM; et. intro T. rewrite U in *. inv T.
+      unfold unwrapU. unfold Mem.store.
+      assert(exists _perm_some, Mem.cnts mem_tgt b 0 = Some _perm_some).
+      { admit "this is simple hack to mimic permission (to give UB properly);
+               should handle it better later". }
+      des. des_ifs.
+      repeat (go; igo). unfold MPut. repeat (go; igo).
+      pfold. econs; ss; et.
+      { esplits; ss; et. ii. ss. unfold mem_src'. des_ifs; bsimpl; des; des_sumbool; des_ifs.
+        econs; et. }
+    }
+  Unshelve.
+    all: ss.
+    all: try (by repeat econs; et).
+  Unshelve.
+    all: try (by repeat econs; et).
+  Qed.
   (* Theorem correct: ModSemPair.sim Mem1.MemSem Mem0.MemSem. *)
   (* Proof. *)
   (*   econstructor 1 with (wf:=wf) (le:=top2); et; swap 2 3. *)
